theories/common/AstCommon.v
@@ -1,5 +1,4 @@
 
-Add LoadPath "../../../template-coq-coq-8.5-coqOpam/theories" as Template.
 Add LoadPath "../common" as Common.
 
 Require Export Template.Ast.
